src/Helpers/FinMap.v
@@ -1,0 +1,470 @@
+(* a finite partial map *)
+
+Require Import Arith.
+Require Import Omega.
+Require Import FunctionalExtensionality.
+Require Import ProofIrrelevance.
+
+Set Implicit Arguments.
+
+Module Map.
+  Section Map.
+    Notation A := nat.
+    Infix "==" := Nat.eq_dec (no associativity, at level 30).
+
+    Variable V:Type.
+
+    Local Record t :=
+      { get :> A -> option V;
+        max : nat;
+        mapping_finite : forall a, max < a -> get a = None;
+        max_minimal : (get max <> None) \/ max = 0 }.
+
+    Hint Extern 4 (_ < _) => omega.
+    Hint Resolve mapping_finite.
+    Hint Extern 2 (_ <> _) => congruence.
+    Hint Extern 2 (_ = _ -> False) => congruence.
+    Hint Resolve max_minimal.
+
+    Fixpoint lower_mapping (x:t) n : A :=
+      match n with
+      | 0 => 0
+      | S n' => match x n' with
+               | Some _ => n'
+               | None => lower_mapping x n'
+               end
+      end.
+
+    Theorem lower_mapping_smaller : forall x n,
+        lower_mapping x n < n \/ n = 0.
+    Proof.
+      induction n; simpl; auto.
+      destruct (x n); intuition auto.
+      subst; auto.
+    Qed.
+
+    Theorem lower_mapping_not_none : forall (x:t) n,
+        x (lower_mapping x n) <> None \/
+        lower_mapping x n = 0.
+    Proof.
+      induction n; simpl; auto.
+      destruct_with_eqn (x n); intuition auto.
+    Qed.
+
+    Theorem lower_mapping_maximal : forall x n,
+        forall a, lower_mapping x n < a -> a < n -> x a = None.
+    Proof.
+      intros.
+      induction n; simpl in *; intros.
+      exfalso; omega.
+      destruct_with_eqn (x n); auto.
+      destruct (a == n); subst; auto.
+    Qed.
+
+    Definition upd (x:t) (a:A) (v:option V) : t.
+      refine {| get :=
+                  fun a' => if a == a' then v else x a';
+                max :=
+                  if lt_dec (max x) a then
+                    (* modification past current end *)
+                    match v with
+                    | Some _ => a
+                    | None => max x (* no-op *)
+                    end else
+                    match v with
+                    | Some _ => max x
+                    | None => (* deleting from the middle; might need to lower max *)
+                        if a == max x then
+                          lower_mapping x (max x) else
+                          max x
+                    end|};
+        intros.
+      - destruct (lt_dec (max x) a), (a == a0), v; subst; try omega; auto.
+        destruct (a == max x); subst; auto.
+        destruct (lt_dec a0 (max x)); auto.
+        apply lower_mapping_maximal with (n := max x); auto.
+      - destruct (lt_dec (max x) a), v; subst;
+          repeat match goal with
+                 | |- context[if ?a == ?b then _ else _] => destruct (a == b)
+                 end; subst; try omega; auto.
+        destruct (lower_mapping_smaller x (max x)); try omega.
+        rewrite H; simpl; auto.
+        destruct (lower_mapping_not_none x (max x)); auto.
+    Defined.
+
+    Theorem t_ext_eq : forall (x y:t),
+        (forall a, x a = y a) ->
+        x = y.
+    Proof.
+      intros.
+      destruct x as [x x_max mapping_finite_x max_minimal_x].
+      destruct y as [y y_max mapping_finite_y max_minimal_y].
+      simpl in *.
+      assert (x = y).
+      extensionality a; auto.
+      subst y.
+      clear H.
+      assert (x_max = y_max). { (* the main proof *)
+        destruct max_minimal_x, max_minimal_y; subst; auto.
+        - assert (~x_max < y_max) by (intro; eauto).
+          assert (~y_max < x_max) by (intro; eauto).
+          omega.
+        - specialize (mapping_finite_y x_max).
+          destruct x_max; auto.
+          exfalso; auto.
+        - specialize (mapping_finite_x y_max).
+          destruct y_max; auto.
+          exfalso; auto.
+      }
+      subst.
+      f_equal; auto using proof_irrelevance.
+    Qed.
+
+    Ltac t :=
+      intros;
+      try lazymatch goal with
+          | |- @eq t _ _ => apply t_ext_eq; intros
+          end;
+      simpl;
+      repeat match goal with
+             | [ |- context[?a == ?a' ] ] =>
+               destruct (a == a')
+             | _ => congruence
+             end.
+
+    Theorem upd_eq : forall x a v,
+        upd x a v a = v.
+    Proof.
+      t.
+    Qed.
+
+    Theorem upd_ne: forall (x:t) a a' v,
+        a <> a' ->
+        upd x a v a' = x a'.
+    Proof.
+      t.
+    Qed.
+
+    Theorem upd_upd_eq : forall x a v v',
+        upd (upd x a v) a v' = upd x a v'.
+    Proof.
+      t.
+    Qed.
+
+    Theorem upd_ne_comm : forall (x:t) a a' v v',
+        a <> a' ->
+        upd (upd x a v) a' v' = upd (upd x a' v') a v.
+    Proof.
+      t.
+    Qed.
+
+    Theorem upd_same_eq : forall (x:t) a v,
+        x a = v ->
+        upd x a v = x.
+    Proof.
+      t.
+    Qed.
+
+    Theorem upd_max_bound : forall (x:t) a v,
+        a <= max x ->
+        max (upd x a v) <= max x.
+    Proof.
+      simpl; intros.
+      generalize dependent (max x); intros m **.
+      destruct (lt_dec m a).
+      destruct v; auto.
+      destruct v; auto.
+      destruct (a == m); subst; auto.
+      destruct (lower_mapping_smaller x m); subst; auto.
+      omega.
+    Qed.
+
+    Theorem upd_max_extend : forall (x:t) a v,
+        a > max x ->
+        max (upd x a (Some v)) > max x.
+    Proof.
+      simpl; intros.
+      generalize dependent (max x); intros m **.
+      destruct (lt_dec m a); auto.
+    Qed.
+
+    Theorem upd_max_extend_bound : forall (x:t) a v,
+        a >= max x ->
+        max (upd x a v) <= a.
+    Proof.
+      simpl; intros.
+      generalize dependent (max x); intros m **.
+      destruct (lt_dec m a); auto.
+      destruct v; auto; try omega.
+      destruct v; auto; try omega.
+      destruct (a == m); subst; auto.
+      destruct (lower_mapping_smaller x m); subst; auto.
+      omega.
+    Qed.
+
+    Theorem upd_max_shrink : forall (x:t) a,
+        max (upd x a None) <= max x.
+    Proof.
+      simpl; intros.
+      generalize dependent (max x); intros m **.
+      destruct (lt_dec m a); auto.
+      destruct (a == m); subst; auto.
+      destruct (lower_mapping_smaller x m); subst; auto.
+      omega.
+    Qed.
+
+    Theorem upd_unchanged : forall (x:t) a v,
+        a <= max x ->
+        max (upd x a (Some v)) = max x.
+    Proof.
+    Abort.
+
+    Theorem past_max_empty : forall (x:t),
+        x (1 + max x) = None.
+    Proof.
+      intros.
+      apply mapping_finite; omega.
+    Qed.
+
+    Definition empty : t.
+      refine {| get := fun _ => None;
+                max := 0; |}; auto.
+    Defined.
+
+    Theorem empty_is_empty : forall a,
+        empty a = None.
+    Proof.
+      simpl; auto.
+    Qed.
+
+    Theorem empty_not_some : forall a v,
+        ~empty a = Some v.
+    Proof.
+      simpl; auto.
+    Qed.
+
+    Theorem empty_unique : forall (x:t),
+        (forall a, x a = None) ->
+        x = empty.
+    Proof.
+      t.
+    Qed.
+
+    Theorem empty_max :
+      max empty = 0.
+    Proof.
+      t.
+    Qed.
+
+    Definition Forall (P: V -> Prop) (x:t) :=
+      forall a v, x a = Some v -> P v.
+
+    Theorem Forall_some : forall P x a v,
+        Forall P x ->
+        x a = Some v ->
+        P v.
+    Proof.
+      unfold Forall; eauto.
+    Qed.
+
+    Theorem empty_Forall : forall P,
+        Forall P empty.
+    Proof.
+      unfold Forall; intros.
+      apply empty_not_some in H; contradiction.
+    Qed.
+
+    Theorem Forall_upd_some : forall P x a v,
+        Forall P x ->
+        P v ->
+        Forall P (upd x a (Some v)).
+    Proof.
+      unfold Forall.
+      t.
+      destruct (a == a0); subst;
+        rewrite ?Map.upd_eq, ?Map.upd_ne in * by auto;
+        subst;
+        eauto.
+      congruence.
+    Qed.
+
+    Theorem Forall_forall : forall (P: V -> Prop) (x:t),
+        (forall a v, x a = Some v -> P v) ->
+        Forall P x.
+    Proof.
+      unfold Forall; eauto.
+    Qed.
+
+    Theorem Forall_upd_none : forall P x a,
+        Forall P x ->
+        Forall P (upd x a None).
+    Proof.
+      unfold Forall.
+      t.
+      destruct (a == a0); subst;
+        rewrite ?Map.upd_eq, ?Map.upd_ne in * by auto;
+        subst;
+        eauto.
+      congruence.
+    Qed.
+
+    Definition from_list (l: list V) : t.
+      refine {| get := fun a => List.nth_error l a;
+                max := length l - 1; |}.
+      intros.
+      apply List.nth_error_None; omega.
+      destruct_with_eqn (List.nth_error l (length l - 1)); eauto.
+      right.
+      apply List.nth_error_None in Heqo.
+      omega.
+    Defined.
+
+    Theorem from_list_get : forall l a,
+        from_list l a = List.nth_error l a.
+    Proof.
+      auto.
+    Qed.
+
+    Local Fixpoint _to_list (x:t) n : list (option V) :=
+      match n with
+      | 0 => nil
+      | S n' => _to_list x n' ++ (x n'::nil)
+      end.
+
+    Definition to_list (x:t) : list (option V) := _to_list x (1 + max x).
+
+    Lemma firstn_map : forall A B (f: A -> B) n (l: list A),
+        List.firstn n (List.map f l) = List.map f (List.firstn n l).
+    Proof.
+      induction n; simpl; intros; auto.
+      destruct l; simpl; eauto.
+      rewrite IHn; auto.
+    Qed.
+
+    Lemma nth_error_nil : forall A n,
+        List.nth_error (@nil A) n = None.
+    Proof.
+      induction n; simpl; eauto.
+    Qed.
+
+    (* TODO: prove this, just for fun (note that it is unused; conversion back
+    to lists is only for extraction purposes) *)
+    Lemma from_list__to_list : forall l n,
+        n <= length l ->
+        _to_list (from_list l) n = List.firstn n (List.map Some l).
+    Proof.
+      induction n; intros; auto.
+      cbn [_to_list get from_list].
+      rewrite IHn by omega.
+      rewrite ?firstn_map.
+      clear IHn.
+      fold (lt n (length l)) in H.
+    Admitted.
+
+    Theorem from_list_to_list : forall l,
+        0 < length l ->
+        to_list (from_list l) = List.map Some l.
+    Proof.
+      unfold to_list; intros.
+      unfold to_list.
+      rewrite from_list__to_list by (simpl; omega).
+      rewrite List.firstn_all2; auto.
+      rewrite List.map_length.
+      simpl; omega.
+    Qed.
+
+  End Map.
+
+  Theorem max_eq : forall V1 V2 (x1:t V1) (x2:t V2),
+      (forall a, x1 a = None <-> x2 a = None) ->
+      max x1 = max x2.
+  Proof.
+    (* will do proof by symmetry *)
+    assert (forall V1 V2 (x1:t V1) (x2:t V2),
+               (forall a, x1 a = None <-> x2 a = None) ->
+               max x1 < max x2 -> False).
+    intros.
+    pose proof (@mapping_finite _ x1 (max x2) ltac:(omega)).
+    apply H in H1.
+    destruct (max_minimal x2); try congruence.
+    omega.
+
+    intros.
+    assert (forall a, x2 a = None <-> x1 a = None).
+    split; intuition auto.
+    apply H0; auto.
+    apply H0; auto.
+    pose proof (H _ _ x1 x2).
+    pose proof (H _ _ x2 x1).
+    intuition auto.
+    omega.
+  Qed.
+
+  Section Map_map.
+
+    Variable V1:Type.
+    Variable V2:Type.
+    Variable f:V1 -> V2.
+
+    Definition map (x:t V1) : t V2.
+      refine {| get := fun a => match x a with
+                             | None => None
+                             | Some v => Some (f v)
+                             end;
+                max := max x; |}; intros.
+      destruct_with_eqn (x a); eauto.
+      rewrite mapping_finite in Heqo by auto; congruence.
+
+      destruct (max_minimal x); auto.
+      destruct (x (max x)); auto.
+      left; congruence.
+    Defined.
+
+    Theorem map_get_match : forall (x:t V1) a,
+        map x a = match x a with
+                  | Some v => Some (f v)
+                  | None => None
+                  end.
+    Proof.
+      simpl; auto.
+    Qed.
+
+    Theorem map_get_some : forall (x:t V1) a v,
+        x a = Some v ->
+        map x a = Some (f v).
+    Proof.
+      simpl; intros.
+      rewrite H; auto.
+    Qed.
+
+    Theorem map_get_none : forall (x:t V1) a,
+        x a = None ->
+        map x a = None.
+    Proof.
+      simpl; intros.
+      rewrite H; auto.
+    Qed.
+
+    Theorem map_Forall : forall (P: V1 -> Prop) (Q:V2 -> Prop) (x:t V1),
+        Forall P x ->
+        (forall v, P v -> Q (f v)) ->
+        Forall Q (map x).
+    Proof.
+      unfold Forall; simpl; intros.
+      destruct_with_eqn (x a).
+      inversion H1; subst; eauto.
+      congruence.
+    Qed.
+
+  End Map_map.
+
+End Map.
+
+Global Opaque Map.get Map.upd Map.empty Map.Forall Map.from_list Map.map.
+
+Hint Rewrite Map.upd_eq : upd.
+Hint Rewrite Map.upd_ne using solve [ auto ] : upd.
+Hint Rewrite Map.upd_upd_eq : upd.
+Hint Rewrite Map.upd_same_eq using solve [ auto ] : upd.
+Hint Rewrite Map.map_get_none using solve [ auto ] : upd.
+Hint Rewrite Map.empty_max : upd.
