src/Spec/ProcMatch.v
@@ -1,0 +1,255 @@
+Require Import Spec.ConcurProc.
+Require Import Spec.Equiv.
+Require Import Helpers.Helpers.
+Require Import Helpers.FinMap.
+
+Require Import Omega.
+
+(** Helpers for connecting different [threads_state]s *)
+
+Definition proc_match `(R : forall T, proc opT T -> proc opT' T -> Prop)
+                      `(ts1 : @threads_state opT)
+                      `(ts2 : @threads_state opT') :=
+  forall tid,
+    match ts1 tid with
+    | Proc p1 =>
+      (* needs to be an exists since need type of ts2 tid to be T *)
+      exists p2, ts2 tid = Proc p2 /\
+            R _ p1 p2
+    | NoProc => ts2 tid = NoProc
+    end.
+
+Theorem proc_match_sym : forall `(R : forall T, proc opT T -> proc opT' T -> Prop)
+                           ts1 ts2,
+    proc_match R ts1 ts2 ->
+    proc_match (fun T x y => R T y x) ts2 ts1.
+Proof.
+  unfold proc_match; intros.
+  specialize (H tid).
+  destruct_with_eqn (ts1 tid); propositional;
+    replace (ts2 tid);
+    eauto.
+Qed.
+
+Theorem proc_match_subrelation : forall opT opT'
+                                   (R1 R2: forall T, proc opT T -> proc opT' T -> Prop)
+                                   ts1 ts2,
+    proc_match R1 ts1 ts2 ->
+    (forall T p1 p2, R1 T p1 p2 -> R2 T p1 p2) ->
+    proc_match R2 ts1 ts2.
+Proof.
+  unfold proc_match; intros.
+  specialize (H tid); destruct matches in *; propositional; eauto.
+Qed.
+
+Theorem proc_match_max_eq : forall `(R : forall T, proc opT T -> proc opT' T -> Prop)
+                           ts1 ts2,
+    proc_match R ts1 ts2 ->
+    Map.max ts1 = Map.max ts2.
+Proof.
+  intros.
+  apply thread_max_eq; intros.
+  specialize (H tid).
+  destruct_with_eqn (ts1 tid); propositional;
+    (intuition auto);
+    congruence.
+Qed.
+
+Lemma proc_match_del : forall `(ts1 : @threads_state opT)
+                              `(ts2 : @threads_state opT') R tid,
+  proc_match R ts1 ts2 ->
+  proc_match R (ts1 [[ tid := NoProc ]]) (ts2 [[ tid := NoProc ]]).
+Proof.
+  unfold proc_match; intros.
+  specialize (H tid0).
+  destruct (tid == tid0); subst;
+    autorewrite with t; eauto.
+Qed.
+
+Lemma proc_match_upd : forall `(ts1 : @threads_state opT)
+                              `(ts2 : @threads_state opT') R tid
+                              T (p1 : proc _ T) p2,
+  proc_match R ts1 ts2 ->
+  R _ p1 p2 ->
+  proc_match R (ts1 [[ tid := Proc p1 ]]) (ts2 [[ tid := Proc p2 ]]).
+Proof.
+  unfold proc_match; intros.
+  specialize (H tid0).
+  destruct (tid == tid0); subst;
+    autorewrite with t;
+    eauto.
+Qed.
+
+Lemma proc_match_nil : forall `(R : forall T, proc opT T -> proc opT' T -> Prop),
+  proc_match R threads_empty threads_empty.
+Proof.
+  unfold proc_match; intros.
+  rewrite ?threads_empty_get; eauto.
+Qed.
+
+Theorem proc_match_pick : forall tid `(ts1 : @threads_state opT)
+                                     `(ts2 : @threads_state opT') R,
+  proc_match R ts1 ts2 ->
+    (ts1 [[ tid ]] = NoProc /\ ts2 [[ tid ]] = NoProc) \/
+    exists T (p1 : proc _ T) p2,
+    ts1 [[ tid ]] = Proc p1 /\ ts2 [[ tid ]] = Proc p2 /\ R T p1 p2.
+Proof.
+  unfold proc_match; intros.
+  specialize (H tid).
+  destruct_with_eqn (ts1 tid); propositional; eauto 10.
+Qed.
+
+Theorem proc_match_trans : forall `(ts1: @threads_state opT)
+                            `(ts2: @threads_state opT') R1
+                            `(ts3: @threads_state opT'') R2,
+  proc_match R1 ts1 ts2 ->
+  proc_match R2 ts2 ts3 ->
+  proc_match (fun T x z => exists y, R1 T x y /\ R2 T y z)  ts1 ts3.
+Proof.
+  unfold proc_match; intros.
+  specialize (H tid).
+  specialize (H0 tid).
+  destruct matches in *;
+    propositional;
+    repeat simpl_match; repeat maybe_proc_inv; eauto 10.
+Qed.
+
+Theorem proc_match_map : forall `(ts1: @threads_state opT)
+                           `(f: forall T, proc opT T -> proc opT' T),
+    proc_match (fun T p1 p2 => p2 = f T p1) ts1 (thread_map f ts1).
+Proof.
+  unfold proc_match; intros.
+  rewrite thread_map_get.
+  destruct matches; propositional; repeat simpl_match; eauto.
+Qed.
+
+Theorem proc_match_map1 : forall `(ts1: @threads_state opT)
+                            `(f: forall T, proc opT T -> proc opT' T)
+                            `(ts2: @threads_state opT'') R,
+    proc_match (fun T p1 p2 => R T (f T p1) p2) ts1 ts2 ->
+    proc_match R (thread_map f ts1) ts2.
+Proof.
+  intros.
+  unfold proc_match; intros.
+  rewrite thread_map_get.
+  specialize (H tid).
+  destruct matches; propositional; repeat simpl_match; eauto.
+Qed.
+
+Theorem proc_match_map2 : forall `(ts1: @threads_state opT)
+                            `(f: forall T, proc opT' T -> proc opT'' T)
+                            `(ts2: @threads_state opT') R,
+    proc_match (fun T p1 p2 => R T p1 (f T p2)) ts1 ts2 ->
+    proc_match R ts1 (thread_map f ts2).
+Proof.
+  intros.
+  unfold proc_match; intros.
+  rewrite thread_map_get.
+  specialize (H tid).
+  destruct_with_eqn (ts1 tid); propositional; repeat simpl_match; eauto.
+Qed.
+
+(** proving equivalence based on per-process equivalence *)
+
+Fixpoint take_threads opT (src: @threads_state opT) n (dst: @threads_state opT) :=
+  match n with
+  | 0 => dst
+  | S n => (take_threads src n dst) [[ n := src n ]]
+  end.
+
+Lemma take_threads_complete_helper : forall opT (src dst: @threads_state opT) n tid,
+    tid < n ->
+    take_threads src n dst tid = src tid.
+Proof.
+  induction n; simpl; intros.
+  - exfalso; omega.
+  - destruct (tid == n); subst;
+      autorewrite with t;
+      eauto.
+    apply IHn; omega.
+Qed.
+
+Lemma take_threads_unchanged_helper : forall opT (src dst: @threads_state opT) n tid,
+    tid >= n ->
+    take_threads src n dst tid = dst tid.
+Proof.
+  induction n; simpl; intros; auto.
+  destruct (tid == n); subst;
+    autorewrite with t.
+  exfalso; omega.
+  apply IHn; omega.
+Qed.
+
+Theorem take_threads_max : forall opT (src dst: @threads_state opT) n,
+    n <= Map.max dst ->
+    Map.max (take_threads src n dst) <= Map.max dst.
+Proof.
+  induction n; simpl; intros.
+  auto.
+  specialize (IHn ltac:(omega)).
+  destruct (le_dec n (Map.max (take_threads src n dst))).
+  rewrite thread_upd_max_bound; auto.
+  rewrite thread_upd_max_extend_bound; omega.
+Qed.
+
+Lemma take_threads_complete_general : forall opT (src dst: @threads_state opT) n,
+    n > Map.max src ->
+    Map.max dst <= Map.max src ->
+    take_threads src n dst = src.
+Proof.
+  intros.
+  apply thread_ext_eq; intros.
+  destruct (lt_dec tid n).
+  apply take_threads_complete_helper; auto.
+  rewrite take_threads_unchanged_helper by omega.
+  rewrite ?thread_mapping_finite by omega.
+  reflexivity.
+Qed.
+
+Theorem take_threads_complete : forall opT (src dst: @threads_state opT),
+    Map.max src = Map.max dst ->
+    src = take_threads src (1 + Map.max src) dst.
+Proof.
+  intros.
+  rewrite take_threads_complete_general; auto; omega.
+Qed.
+
+Lemma take_threads_none : forall opT (src dst: @threads_state opT),
+    dst = take_threads src 0 dst.
+Proof.
+  reflexivity.
+Qed.
+
+Theorem trace_incl_ts_general : forall opT State (op_step: OpSemantics opT State) (ts1 ts2: threads_state),
+    (forall tid, trace_incl_opt op_step (ts1 tid) (ts2 tid)) ->
+    Map.max ts1 = Map.max ts2 ->
+    trace_incl_ts op_step ts1 ts2.
+Proof.
+  intros.
+  rewrite (take_threads_complete ts2 ts1) by auto.
+  generalize dependent (1 + Map.max ts2).
+  induction n; simpl.
+  reflexivity.
+  etransitivity; eauto.
+  replace (take_threads ts2 n ts1) with
+      ((take_threads ts2 n ts1) [[n := ts1 n]]) at 1;
+    swap 1 2.
+  rewrite thread_upd_same_eq; auto.
+  rewrite take_threads_unchanged_helper; auto.
+  generalize dependent (take_threads ts2 n ts1); intros ts' **.
+  apply H.
+Qed.
+
+Theorem trace_incl_ts_proc_match : forall opT State (op_step: OpSemantics opT State) ts1 ts2,
+    proc_match (fun T => trace_incl op_step (T:=T)) ts1 ts2 ->
+    trace_incl_ts op_step ts1 ts2.
+Proof.
+  intros.
+  apply trace_incl_ts_general.
+  - intros.
+    unfold trace_incl in *.
+    specialize (H tid).
+    destruct_with_eqn (ts1 tid); propositional; try congruence.
+    rewrite H in *; auto.
+  - eauto using proc_match_max_eq.
+Qed.
